Add products

STLC3.v
@@ -1,13 +1,17 @@
 Require Export stlc.Maps.
 
 Inductive type : Type := 
-  | tvar  : string -> type 
-  | tarr : type -> type -> type.
+  | tvar : string -> type
+  | tarr : type -> type -> type
+  | tprod : type -> type -> type.
 
 Inductive term : Type :=
   | var : string -> term
   | app : term -> term -> term
-  | lam : string -> type -> term -> term.
+  | lam : string -> type -> term -> term
+  | prod : term -> term -> term
+  | fst : term -> term
+  | snd : term -> term.
 
 Definition ctx := partial_map type.
 
@@ -43,7 +47,17 @@ Inductive typed : ctx -> term -> type -> Prop :=
       typed E (app M N) B
   | lam_typed : forall E x A B M,
       typed (update E x A) M B -> 
-      typed E (lam x A M) (tarr A B).
+      typed E (lam x A M) (tarr A B)
+  | prod_typed : forall E t s T S,
+      typed E t T ->
+      typed E s S ->
+      typed E (prod t s) (tprod T S)
+  | fst_typed : forall E p T S,
+      typed E p (tprod T S) ->
+      typed E (fst p) T
+  | snd_typed : forall E p T S,
+      typed E p (tprod T S) ->
+      typed E (snd p) S.
 
 (* Exercise 2.4 *)
 
@@ -51,11 +65,11 @@ Lemma test : typed  empty
                     (lxly_x "X" "Y") 
                     (X_Y_X "X" "Y").
 Proof.
-unfold lxly_x. unfold X_Y_X.
-apply lam_typed. 
-apply lam_typed. 
-apply var_typed.
-reflexivity.
+  unfold lxly_x. unfold X_Y_X.
+  apply lam_typed. 
+  apply lam_typed. 
+  apply var_typed.
+  reflexivity.
 Qed.
 
 (* Exercise 2.5 *)
@@ -66,8 +80,10 @@ Qed.
 Fixpoint beq_type (A B:type) : bool :=
   match A,B with
   | tvar a, tvar b => beq_string a b
-  | tarr A1 A2, tarr B1 B2 =>
-      andb (beq_type A1 B1) (beq_type A2 B2)
+  | tarr A1 B1, tarr A2 B2 =>
+      andb (beq_type A1 A2) (beq_type B1 B2)
+  | tprod T1 S1, tprod T2 S2 => 
+      andb (beq_type T1 T2) (beq_type S1 S2)
   | _,_ => 
       false
   end.
@@ -77,7 +93,8 @@ Lemma beq_type_refl : forall A,
 Proof.
   intros A1. induction A1; simpl.
   apply beq_string_true_iff. reflexivity.
-  rewrite IHA1_1. rewrite IHA1_2. reflexivity.  Qed.
+  rewrite IHA1_1. rewrite IHA1_2. reflexivity.
+  rewrite IHA1_1. rewrite IHA1_2. reflexivity. Qed.
 
 Lemma beq_type_eq : forall A B,
   beq_type A B = true -> A = B.
@@ -85,20 +102,41 @@ Proof.
   intros A. induction A; intros A Hbeq; destruct A; inversion Hbeq.
   - apply beq_string_true_iff in H0. rewrite H0. reflexivity.
   - apply andb_prop in H0. inversion H0 as [Hbeq1 Hbeq2].
-    apply IHA1 in Hbeq1. apply IHA2 in Hbeq2. subst... reflexivity. Qed.
+    apply IHA1 in Hbeq1. apply IHA2 in Hbeq2. subst... reflexivity.
+  - apply andb_prop in H0. inversion H0 as [Hbeq1 Hbeq2].
+    apply IHA1 in Hbeq1. apply IHA2 in Hbeq2. subst... reflexivity.
+Qed.
 
 Fixpoint typecheck (E:ctx) (t:term) : option type :=
   match t with
-  | var x     => E x
-  | app M N   => match typecheck E M, typecheck E N with
-                 | Some (tarr A B),Some A1 =>
-                    if beq_type A A1 then Some B else None
-                 | _,_ => None
-                    end
-  | lam x A M => match typecheck (update E x A) M with
-                 | Some B => Some (tarr A B)
-                 | _ => None
-                 end
+  | var x => 
+      E x
+  | app M N => 
+      match typecheck E M, typecheck E N with
+      | Some (tarr A B),Some A1 =>
+          if beq_type A A1 then Some B else None
+      | _,_ => None
+      end
+  | lam x A M => 
+      match typecheck (update E x A) M with
+      | Some B => Some (tarr A B)
+      | _ => None
+      end
+  | prod s t => 
+      match typecheck E s, typecheck E t with
+      | Some A, Some B => Some (tprod A B)
+      | _,_ => None
+      end
+  | fst p => 
+      match typecheck E p with
+      | Some (tprod A B) => Some A
+      | _ => None
+      end
+  | snd p => 
+      match typecheck E p with
+      | Some (tprod A B) => Some B
+      | _ => None
+      end
   end.
 
 (* Exercise 2.6 *)
@@ -114,7 +152,7 @@ nothing if there is no type).
 (* Exercise 2.7 *)
 
 Example pos_typecheck_1 : 
-typecheck empty (lxly_x "X" "Y") = Some (X_Y_X "X" "Y").
+  typecheck empty (lxly_x "X" "Y") = Some (X_Y_X "X" "Y").
 Proof. reflexivity. Qed.
 
 Example pos_typecheck_2 : 
@@ -143,24 +181,23 @@ Lemma typecheck_complete : forall E t A,
   typed E t A ->
   typecheck E t = Some A.
 Proof.
-intros E t A H.
-induction H.
-- apply H.
-- simpl.
-  rewrite IHtyped1. rewrite IHtyped2.
-  rewrite beq_type_refl.
-  reflexivity.
-- simpl.
-  rewrite IHtyped. reflexivity.
+  intros E t A H.
+  induction H.
+  - apply H.
+  - simpl.
+    rewrite IHtyped1. rewrite IHtyped2.
+    rewrite beq_type_refl.
+    reflexivity.
+  - simpl.
+    rewrite IHtyped. reflexivity.
+  - simpl.
+    rewrite IHtyped1. rewrite IHtyped2.
+    reflexivity.
+  - simpl.
+    rewrite IHtyped. reflexivity.
+  - simpl.
+    rewrite IHtyped. reflexivity.
 Qed.
-
-Ltac solve_by_invert :=
-  match goal with 
-  | H : ?T 
-  |- _ => match type of T with 
-          | Prop => solve [inversion H]
-          end
-  end.
 
 Lemma typecheck_sound : forall E t A,
   typecheck E t = Some A -> typed E t A.
@@ -170,11 +207,11 @@ Proof.
   - apply var_typed. apply H0.
   - remember (typecheck E t1) as TO1.
     remember (typecheck E t2) as TO2.
-    destruct TO1 as [A|]; try solve_by_invert;
-    destruct A as [|A1 A2]; try solve_by_invert.
-    destruct TO2 as [B|]; try solve_by_invert.
+    destruct TO1 as [A|]; inversion H0;
+    destruct A as [|A1 A2|T1 S1]; inversion H0.
+    destruct TO2 as [B|]; inversion H0.
     remember (beq_type A1 B) as b.
-    destruct b; try solve_by_invert.
+    destruct b; inversion H0.
     symmetry in Heqb. apply beq_type_eq in Heqb.
     inversion H0; subst... 
     apply app_typed with (A := B) (B := T).
@@ -184,17 +221,59 @@ Proof.
     apply IHt2 in HeqTO2. apply HeqTO2.
   - remember (update E s t) as G'.
     remember (typecheck G' t0) as TO2.
-    destruct TO2; try solve_by_invert.
+    destruct TO2; inversion H0.
     inversion H0. apply lam_typed. rewrite <- HeqG'.
-    apply IHt. rewrite HeqTO2. reflexivity. Qed.
+    apply IHt. rewrite HeqTO2. reflexivity. 
+  - remember (typecheck E t1) as TO1.
+    remember (typecheck E t2) as TO2.
+    destruct TO1; inversion H0.
+    destruct TO2; inversion H0.
+    apply prod_typed.
+    symmetry in HeqTO1. apply IHt1 in HeqTO1.
+    apply HeqTO1.
+    symmetry in HeqTO2. apply IHt2 in HeqTO2.
+    apply HeqTO2.
+  - remember (typecheck E t) as TO1.
+    destruct TO1; inversion H0.
+    destruct t0; inversion H0.
+    symmetry in HeqTO1.
+    apply IHt in HeqTO1.
+    rewrite -> H2 in HeqTO1.
+    apply fst_typed with (S := t0_2).
+    apply HeqTO1.
+  - remember (typecheck E t) as TO1.
+    destruct TO1; inversion H0.
+    destruct t0; inversion H0.
+    symmetry in HeqTO1.
+    apply IHt in HeqTO1.
+    rewrite -> H2 in HeqTO1.
+    apply snd_typed with (T := t0_1).
+    apply HeqTO1.
+Qed.
 
+(*
+Inductive typed : ctx -> term -> type -> Prop :=
+  | var_typed : forall E x A,
+      E x = Some A ->
+      typed E (var x) A
+  | app_typed : forall A B E M N,
+      typed E M (tarr A B) ->
+      typed E N A -> 
+      typed E (app M N) B
+  | lam_typed : forall E x A B M,
+      typed (update E x A) M B -> 
+      typed E (lam x A M) (tarr A B)
+  | prod_typed : forall E t s T S,
+      typed E t T ->
+      typed E s S ->
+      typed E (prod t s) (tprod T S)
+  | fst_typed : forall E p T S,
+      typed E p (tprod T S) ->
+      typed E (fst p) T
+  | snd_typed : forall E p T S,
+      typed E p (tprod T S) ->
+      typed E (snd p) S.
 
-
-
-
-
-
-
-
+*)
 
 
